Invariants over states in WP and get rid of heap_ctx.
The WP construction now takes an invariant on states as a parameter
(part of the irisG class) and no longer builds in the authoritative
ownership of the entire state. When instantiating WP with a concrete
language on can choose its state invariant. For example, for heap_lang
we directly use `auth (gmap loc (frac * dec_agree val))`, and avoid
the indirection through invariants entirely.

As a result, we no longer have to carry `heap_ctx` around.

heap_lang/heap.v
@@ -1,39 +1,40 @@
 From iris.heap_lang Require Export lifting.
 From iris.algebra Require Import auth gmap frac dec_agree.
 From iris.base_logic.lib Require Export invariants.
-From iris.base_logic.lib Require Import wsat auth fractional.
+From iris.base_logic.lib Require Import fractional.
+From iris.program_logic Require Import ectx_lifting.
 From iris.proofmode Require Import tactics.
 Import uPred.
 (* TODO: The entire construction could be generalized to arbitrary languages that have
    a finmap as their state. Or maybe even beyond "as their state", i.e. arbitrary
    predicates over finmaps instead of just ownP. *)
 
-Definition heapN : namespace := nroot .@ "heap".
 Definition heapUR : ucmraT := gmapUR loc (prodR fracR (dec_agreeR val)).
+Definition to_heap : state → heapUR := fmap (λ v, (1%Qp, DecAgree v)).
 
 (** The CMRA we need. *)
 Class heapG Σ := HeapG {
-  heapG_iris_inG :> irisG heap_lang Σ;
-  heap_inG :> authG Σ heapUR;
+  heapG_invG : invG Σ;
+  heap_inG :> inG Σ (authR heapUR);
   heap_name : gname
 }.
-
-Definition to_heap : state → heapUR := fmap (λ v, (1%Qp, DecAgree v)).
+Instance heapG_irisG `{heapG Σ} : irisG heap_lang Σ := {
+  iris_invG := heapG_invG;
+  state_interp σ := own heap_name (● to_heap σ)
+}.
 
 Section definitions.
   Context `{heapG Σ}.
 
   Definition heap_mapsto_def (l : loc) (q : Qp) (v: val) : iProp Σ :=
-    auth_own heap_name ({[ l := (q, DecAgree v) ]}).
+    own heap_name (◯ {[ l := (q, DecAgree v) ]}).
   Definition heap_mapsto_aux : { x | x = @heap_mapsto_def }. by eexists. Qed.
   Definition heap_mapsto := proj1_sig heap_mapsto_aux.
   Definition heap_mapsto_eq : @heap_mapsto = @heap_mapsto_def :=
     proj2_sig heap_mapsto_aux.
-
-  Definition heap_ctx : iProp Σ := auth_ctx heap_name heapN to_heap ownP.
 End definitions.
 
-Typeclasses Opaque heap_ctx heap_mapsto.
+Typeclasses Opaque heap_mapsto.
 
 Notation "l ↦{ q } v" := (heap_mapsto l q v)
   (at level 20, q at level 50, format "l  ↦{ q }  v") : uPred_scope.
@@ -42,6 +43,11 @@ Notation "l ↦ v" := (heap_mapsto l 1 v) (at level 20) : uPred_scope.
 Notation "l ↦{ q } -" := (∃ v, l ↦{q} v)%I
   (at level 20, q at level 50, format "l  ↦{ q }  -") : uPred_scope.
 Notation "l ↦ -" := (l ↦{1} -)%I (at level 20) : uPred_scope.
+
+Local Hint Extern 0 (head_reducible _ _) => eexists _, _, _; simpl.
+Local Hint Constructors head_step.
+Local Hint Resolve alloc_fresh.
+Local Hint Resolve to_of_val.
 
 Section heap.
   Context {Σ : gFunctors}.
@@ -62,11 +68,6 @@ Section heap.
     move: Hl. rewrite /to_heap lookup_fmap fmap_Some=> -[v' [Hl [??]]]; subst.
     by move: Hqv=> /Some_pair_included_total_2 [_ /DecAgree_included ->].
   Qed.
-  Lemma heap_singleton_included' σ l q v :
-    {[l := (q, DecAgree v)]} ≼ to_heap σ → to_heap σ !! l = Some (1%Qp,DecAgree v).
-  Proof.
-    intros Hl%heap_singleton_included. by rewrite /to_heap lookup_fmap Hl.
-  Qed.
   Lemma to_heap_insert l v σ :
     to_heap (<[l:=v]> σ) = <[l:=(1%Qp, DecAgree v)]> (to_heap σ).
   Proof. by rewrite /to_heap fmap_insert. Qed.
@@ -74,26 +75,22 @@ Section heap.
   Context `{heapG Σ}.
 
   (** General properties of mapsto *)
-  Global Instance heap_ctx_persistent : PersistentP heap_ctx.
-  Proof. rewrite /heap_ctx. apply _. Qed.
   Global Instance heap_mapsto_timeless l q v : TimelessP (l ↦{q} v).
   Proof. rewrite heap_mapsto_eq /heap_mapsto_def. apply _. Qed.
   Global Instance heap_mapsto_fractional l v : Fractional (λ q, l ↦{q} v)%I.
   Proof.
-    unfold Fractional; intros.
-    by rewrite heap_mapsto_eq -auth_own_op op_singleton pair_op dec_agree_idemp.
+    intros p q. by rewrite heap_mapsto_eq -own_op -auth_frag_op
+      op_singleton pair_op dec_agree_idemp.
   Qed.
   Global Instance heap_mapsto_as_fractional l q v :
     AsFractional (l ↦{q} v) (λ q, l ↦{q} v)%I q.
   Proof. done. Qed.
 
-  Lemma heap_mapsto_agree l q1 q2 v1 v2 :
-    l ↦{q1} v1 ∗ l ↦{q2} v2 ⊢ ⌜v1 = v2⌝.
+  Lemma heap_mapsto_agree l q1 q2 v1 v2 : l ↦{q1} v1 ∗ l ↦{q2} v2 ⊢ ⌜v1 = v2⌝.
   Proof.
-    rewrite heap_mapsto_eq -auth_own_op auth_own_valid discrete_valid
-            op_singleton singleton_valid.
-    f_equiv. move=>[_ ] /=.
-    destruct (decide (v1 = v2)) as [->|?]; first done. by rewrite dec_agree_ne.
+    rewrite heap_mapsto_eq -own_op -auth_frag_op own_valid discrete_valid.
+    f_equiv=> /auth_own_valid /=. rewrite op_singleton singleton_valid pair_op.
+    by move=> [_ /= /dec_agree_op_inv [?]].
   Qed.
 
   Global Instance heap_ex_mapsto_fractional l : Fractional (λ q, l ↦{q} -)%I.
@@ -109,8 +106,8 @@ Section heap.
 
   Lemma heap_mapsto_valid l q v : l ↦{q} v ⊢ ✓ q.
   Proof.
-    rewrite heap_mapsto_eq /heap_mapsto_def auth_own_valid !discrete_valid.
-    by apply pure_mono=> /singleton_valid [??].
+    rewrite heap_mapsto_eq /heap_mapsto_def own_valid !discrete_valid.
+    by apply pure_mono=> /auth_own_valid /singleton_valid [??].
   Qed.
   Lemma heap_mapsto_valid_2 l q1 q2 v1 v2 :
     l ↦{q1} v1 ∗ l ↦{q2} v2 ⊢ ✓ (q1 + q2)%Qp.
@@ -121,74 +118,80 @@ Section heap.
 
   (** Weakest precondition *)
   Lemma wp_alloc E e v :
-    to_val e = Some v → ↑heapN ⊆ E →
-    {{{ heap_ctx }}} Alloc e @ E {{{ l, RET LitV (LitLoc l); l ↦ v }}}.
+    to_val e = Some v →
+    {{{ True }}} Alloc e @ E {{{ l, RET LitV (LitLoc l); l ↦ v }}}.
   Proof.
-    iIntros (<-%of_to_val ? Φ) "#Hinv HΦ". rewrite /heap_ctx.
-    iMod (auth_empty heap_name) as "Ha".
-    iMod (auth_open with "[$Hinv $Ha]") as (σ) "(%&Hσ&Hcl)"; first done.
-    iApply (wp_alloc_pst with "Hσ"). iNext. iIntros (l) "[% Hσ]".
-    iMod ("Hcl" with "* [Hσ]") as "Ha".
-    { iFrame. iPureIntro. rewrite to_heap_insert.
-      eapply alloc_singleton_local_update; by auto using lookup_to_heap_None. }
+    iIntros (<-%of_to_val Φ) "HΦ". iApply wp_lift_atomic_head_step_no_fork; auto.
+    iIntros (σ1) "Hσ !>"; iSplit; first by auto.
+    iNext; iIntros (v2 σ2 efs Hstep); inv_head_step.
+    iMod (own_update with "Hσ") as "[Hσ Hl]".
+    { eapply auth_update_alloc,
+        (alloc_singleton_local_update _ _ (1%Qp, DecAgree _))=> //.
+      by apply lookup_to_heap_None. }
+    iModIntro; iSplit=> //. rewrite to_heap_insert. iFrame.
     iApply "HΦ". by rewrite heap_mapsto_eq /heap_mapsto_def.
   Qed.
 
   Lemma wp_load E l q v :
-    ↑heapN ⊆ E →
-    {{{ heap_ctx ∗ ▷ l ↦{q} v }}} Load (Lit (LitLoc l)) @ E
-    {{{ RET v; l ↦{q} v }}}.
+    {{{ ▷ l ↦{q} v }}} Load (Lit (LitLoc l)) @ E {{{ RET v; l ↦{q} v }}}.
   Proof.
-    iIntros (? Φ) "[#Hinv >Hl] HΦ".
-    rewrite /heap_ctx heap_mapsto_eq /heap_mapsto_def.
-    iMod (auth_open with "[$Hinv $Hl]") as (σ) "(%&Hσ&Hcl)"; first done.
-    iApply (wp_load_pst _ σ with "Hσ"); first eauto using heap_singleton_included.
-    iNext; iIntros "Hσ".
-    iMod ("Hcl" with "* [Hσ]") as "Ha"; first eauto. by iApply "HΦ".
+    iIntros (Φ) ">Hl HΦ". rewrite heap_mapsto_eq /heap_mapsto_def.
+    iApply wp_lift_atomic_head_step_no_fork; auto.
+    iIntros (σ1) "Hσ !>". iDestruct (own_valid_2 with "Hσ Hl")
+      as %[?%heap_singleton_included _]%auth_valid_discrete_2.
+    iSplit; first by eauto.
+    iNext; iIntros (v2 σ2 efs Hstep); inv_head_step.
+    iModIntro; iSplit=> //. iFrame. by iApply "HΦ".
   Qed.
 
   Lemma wp_store E l v' e v :
-    to_val e = Some v → ↑heapN ⊆ E →
-    {{{ heap_ctx ∗ ▷ l ↦ v' }}} Store (Lit (LitLoc l)) e @ E
-    {{{ RET LitV LitUnit; l ↦ v }}}.
+    to_val e = Some v →
+    {{{ ▷ l ↦ v' }}} Store (Lit (LitLoc l)) e @ E {{{ RET LitV LitUnit; l ↦ v }}}.
   Proof.
-    iIntros (<-%of_to_val ? Φ) "[#Hinv >Hl] HΦ".
-    rewrite /heap_ctx heap_mapsto_eq /heap_mapsto_def.
-    iMod (auth_open with "[$Hinv $Hl]") as (σ) "(%&Hσ&Hcl)"; first done.
-    iApply (wp_store_pst _ σ with "Hσ"); first eauto using heap_singleton_included.
-    iNext; iIntros "Hσ". iMod ("Hcl" with "* [Hσ]") as "Ha".
-    { iFrame. iPureIntro. rewrite to_heap_insert.
-      eapply singleton_local_update, exclusive_local_update; last done.
-      by eapply heap_singleton_included'. }
-    by iApply "HΦ".
+    iIntros (<-%of_to_val Φ) ">Hl HΦ". rewrite heap_mapsto_eq /heap_mapsto_def.
+    iApply wp_lift_atomic_head_step_no_fork; auto.
+    iIntros (σ1) "Hσ !>". iDestruct (own_valid_2 with "Hσ Hl")
+      as %[Hl%heap_singleton_included _]%auth_valid_discrete_2.
+    iSplit; first by eauto.
+    iNext; iIntros (v2 σ2 efs Hstep); inv_head_step.
+    iMod (own_update_2 with "Hσ Hl") as "[Hσ1 Hl]".
+    { eapply auth_update, singleton_local_update,
+        (exclusive_local_update _ (1%Qp, DecAgree _))=> //.
+      by rewrite /to_heap lookup_fmap Hl. }
+    iModIntro. iSplit=>//. rewrite to_heap_insert. iFrame. by iApply "HΦ".
   Qed.
 
   Lemma wp_cas_fail E l q v' e1 v1 e2 v2 :
-    to_val e1 = Some v1 → to_val e2 = Some v2 → v' ≠ v1 → ↑heapN ⊆ E →
-    {{{ heap_ctx ∗ ▷ l ↦{q} v' }}} CAS (Lit (LitLoc l)) e1 e2 @ E
+    to_val e1 = Some v1 → to_val e2 = Some v2 → v' ≠ v1 →
+    {{{ ▷ l ↦{q} v' }}} CAS (Lit (LitLoc l)) e1 e2 @ E
     {{{ RET LitV (LitBool false); l ↦{q} v' }}}.
   Proof.
-    iIntros (<-%of_to_val <-%of_to_val ?? Φ) "[#Hinv >Hl] HΦ".
-    rewrite /heap_ctx heap_mapsto_eq /heap_mapsto_def.
-    iMod (auth_open with "[$Hinv $Hl]") as (σ) "(%&Hσ&Hcl)"; first done.
-    iApply (wp_cas_fail_pst _ σ with "Hσ"); [eauto using heap_singleton_included|done|].
-    iNext; iIntros "Hσ".
-    iMod ("Hcl" with "* [Hσ]") as "Ha"; first eauto. by iApply "HΦ".
+    iIntros (<-%of_to_val <-%of_to_val ? Φ) ">Hl HΦ".
+    rewrite heap_mapsto_eq /heap_mapsto_def.
+    iApply wp_lift_atomic_head_step_no_fork; auto.
+    iIntros (σ1) "Hσ !>". iDestruct (own_valid_2 with "Hσ Hl")
+      as %[?%heap_singleton_included _]%auth_valid_discrete_2.
+    iSplit; first by eauto.
+    iNext; iIntros (v2' σ2 efs Hstep); inv_head_step. (* FIXME: this inversion is slow *)
+    iModIntro; iSplit=> //. iFrame. by iApply "HΦ".
   Qed.
 
   Lemma wp_cas_suc E l e1 v1 e2 v2 :
-    to_val e1 = Some v1 → to_val e2 = Some v2 → ↑heapN ⊆ E →
-    {{{ heap_ctx ∗ ▷ l ↦ v1 }}} CAS (Lit (LitLoc l)) e1 e2 @ E
+    to_val e1 = Some v1 → to_val e2 = Some v2 →
+    {{{ ▷ l ↦ v1 }}} CAS (Lit (LitLoc l)) e1 e2 @ E
     {{{ RET LitV (LitBool true); l ↦ v2 }}}.
   Proof.
-    iIntros (<-%of_to_val <-%of_to_val ? Φ) "[#Hinv >Hl] HΦ".
-    rewrite /heap_ctx heap_mapsto_eq /heap_mapsto_def.
-    iMod (auth_open with "[$Hinv $Hl]") as (σ) "(%&Hσ&Hcl)"; first done.
-    iApply (wp_cas_suc_pst _ σ with "Hσ"); first by eauto using heap_singleton_included.
-    iNext. iIntros "Hσ". iMod ("Hcl" with "* [Hσ]") as "Ha".
-    { iFrame. iPureIntro. rewrite to_heap_insert.
-      eapply singleton_local_update, exclusive_local_update; last done.
-      by eapply heap_singleton_included'. }
-    by iApply "HΦ".
+    iIntros (<-%of_to_val <-%of_to_val Φ) ">Hl HΦ".
+    rewrite heap_mapsto_eq /heap_mapsto_def.
+    iApply wp_lift_atomic_head_step_no_fork; auto.
+    iIntros (σ1) "Hσ !>". iDestruct (own_valid_2 with "Hσ Hl")
+      as %[Hl%heap_singleton_included _]%auth_valid_discrete_2.
+    iSplit; first by eauto.
+    iNext; iIntros (v2' σ2 efs Hstep); inv_head_step.
+    iMod (own_update_2 with "Hσ Hl") as "[Hσ1 Hl]".
+    { eapply auth_update, singleton_local_update,
+        (exclusive_local_update _ (1%Qp, DecAgree _))=> //.
+      by rewrite /to_heap lookup_fmap Hl. }
+    iModIntro. iSplit=>//. rewrite to_heap_insert. iFrame. by iApply "HΦ".
   Qed.
 End heap.
