heap_lang/lib/ticket_lock.v
@@ -46,12 +46,10 @@ Section proof.
 
   Definition is_lock (γ : gname) (lk : val) (R : iProp Σ) : iProp Σ :=
     (∃ lo ln : loc,
-       ⌜heapN ⊥ N⌝ ∧ heap_ctx ∧
        ⌜lk = (#lo, #ln)%V⌝ ∧ inv N (lock_inv γ lo ln R))%I.
 
   Definition issued (γ : gname) (lk : val) (x : nat) (R : iProp Σ) : iProp Σ :=
     (∃ lo ln: loc,
-       ⌜heapN ⊥ N⌝ ∧ heap_ctx ∧
        ⌜lk = (#lo, #ln)%V⌝ ∧ inv N (lock_inv γ lo ln R) ∧
        own γ (◯ (∅, GSet {[ x ]})))%I.
 
@@ -74,10 +72,9 @@ Section proof.
   Qed.
 
   Lemma newlock_spec (R : iProp Σ) :
-    heapN ⊥ N →
-    {{{ heap_ctx ∗ R }}} newlock #() {{{ lk γ, RET lk; is_lock γ lk R }}}.
+    {{{ R }}} newlock #() {{{ lk γ, RET lk; is_lock γ lk R }}}.
   Proof.
-    iIntros (HN Φ) "(#Hh & HR) HΦ". rewrite -wp_fupd /newlock.
+    iIntros (Φ) "HR HΦ". rewrite -wp_fupd /newlock /=.
     wp_seq. wp_alloc lo as "Hlo". wp_alloc ln as "Hln".
     iMod (own_alloc (● (Excl' 0%nat, ∅) ⋅ ◯ (Excl' 0%nat, ∅))) as (γ) "[Hγ Hγ']".
     { by rewrite -auth_both_op. }
@@ -90,7 +87,7 @@ Section proof.
   Lemma wait_loop_spec γ lk x R :
     {{{ issued γ lk x R }}} wait_loop #x lk {{{ RET #(); locked γ ∗ R }}}.
   Proof.
-    iIntros (Φ) "Hl HΦ". iDestruct "Hl" as (lo ln) "(% & #? & % & #? & Ht)".
+    iIntros (Φ) "Hl HΦ". iDestruct "Hl" as (lo ln) "(% & #? & Ht)".
     iLöb as "IH". wp_rec. subst. wp_let. wp_proj. wp_bind (! _)%E.
     iInv N as (o n) "(Hlo & Hln & Ha)" "Hclose".
     wp_load. destruct (decide (x = o)) as [->|Hneq].
@@ -111,7 +108,7 @@ Section proof.
   Lemma acquire_spec γ lk R :
     {{{ is_lock γ lk R }}} acquire lk {{{ RET #(); locked γ ∗ R }}}.
   Proof.
-    iIntros (ϕ) "Hl HΦ". iDestruct "Hl" as (lo ln) "(% & #? & % & #?)".
+    iIntros (ϕ) "Hl HΦ". iDestruct "Hl" as (lo ln) "[% #?]".
     iLöb as "IH". wp_rec. wp_bind (! _)%E. subst. wp_proj.
     iInv N as (o n) "[Hlo [Hln Ha]]" "Hclose".
     wp_load. iMod ("Hclose" with "[Hlo Hln Ha]") as "_".
@@ -142,8 +139,7 @@ Section proof.
   Lemma release_spec γ lk R :
     {{{ is_lock γ lk R ∗ locked γ ∗ R }}} release lk {{{ RET #(); True }}}.
   Proof.
-    iIntros (Φ) "(Hl & Hγ & HR) HΦ".
-    iDestruct "Hl" as (lo ln) "(% & #? & % & #?)"; subst.
+    iIntros (Φ) "(Hl & Hγ & HR) HΦ". iDestruct "Hl" as (lo ln) "[% #?]"; subst.
     iDestruct "Hγ" as (o) "Hγo".
     rewrite /release. wp_let. wp_proj. wp_proj. wp_bind (! _)%E.
     iInv N as (o' n) "(>Hlo & >Hln & >Hauth & Haown)" "Hclose".
