heap_lang/lib/barrier/proof.v
@@ -38,7 +38,7 @@ Definition barrier_inv (l : loc) (P : iProp Σ) (s : state) : iProp Σ :=
   (l ↦ s ∗ ress (state_to_prop s P) (state_I s))%I.
 
 Definition barrier_ctx (γ : gname) (l : loc) (P : iProp Σ) : iProp Σ :=
-  (⌜heapN ⊥ N⌝ ∗ heap_ctx ∗ sts_ctx γ N (barrier_inv l P))%I.
+  sts_ctx γ N (barrier_inv l P).
 
 Definition send (l : loc) (P : iProp Σ) : iProp Σ :=
   (∃ γ, barrier_ctx γ l P ∗ sts_ownS γ low_states {[ Send ]})%I.
@@ -91,10 +91,9 @@ Qed.
 
 (** Actual proofs *)
 Lemma newbarrier_spec (P : iProp Σ) :
-  heapN ⊥ N →
-  {{{ heap_ctx }}} newbarrier #() {{{ l, RET #l; recv l P ∗ send l P }}}.
+  {{{ True }}} newbarrier #() {{{ l, RET #l; recv l P ∗ send l P }}}.
 Proof.
-  iIntros (HN Φ) "#? HΦ".
+  iIntros (Φ) "HΦ".
   rewrite -wp_fupd /newbarrier /=. wp_seq. wp_alloc l as "Hl".
   iApply ("HΦ" with ">[-]").
   iMod (saved_prop_alloc (F:=idCF) P) as (γ) "#?".
@@ -120,7 +119,7 @@ Lemma signal_spec l P :
   {{{ send l P ∗ P }}} signal #l {{{ RET #(); True }}}.
 Proof.
   rewrite /signal /send /barrier_ctx /=.
-  iIntros (Φ) "(Hs&HP) HΦ"; iDestruct "Hs" as (γ) "[#(%&Hh&Hsts) Hγ]". wp_let.
+  iIntros (Φ) "[Hs HP] HΦ". iDestruct "Hs" as (γ) "[#Hsts Hγ]". wp_let.
   iMod (sts_openS (barrier_inv l P) _ _ γ with "[Hγ]")
     as ([p I]) "(% & [Hl Hr] & Hclose)"; eauto.
   destruct p; [|done]. wp_store.
@@ -136,7 +135,7 @@ Lemma wait_spec l P:
   {{{ recv l P }}} wait #l {{{ RET #(); P }}}.
 Proof.
   rename P into R; rewrite /recv /barrier_ctx.
-  iIntros (Φ) "Hr HΦ"; iDestruct "Hr" as (γ P Q i) "(#(%&Hh&Hsts)&Hγ&#HQ&HQR)".
+  iIntros (Φ) "Hr HΦ"; iDestruct "Hr" as (γ P Q i) "(#Hsts & Hγ & #HQ & HQR)".
   iLöb as "IH". wp_rec. wp_bind (! _)%E.
   iMod (sts_openS (barrier_inv l P) _ _ γ with "[Hγ]")
     as ([p I]) "(% & [Hl Hr] & Hclose)"; eauto.
@@ -165,7 +164,7 @@ Lemma recv_split E l P1 P2 :
   ↑N ⊆ E → recv l (P1 ∗ P2) ={E}=∗ recv l P1 ∗ recv l P2.
 Proof.
   rename P1 into R1; rename P2 into R2. rewrite {1}/recv /barrier_ctx.
-  iIntros (?). iDestruct 1 as (γ P Q i) "(#(%&Hh&Hsts)&Hγ&#HQ&HQR)".
+  iIntros (?). iDestruct 1 as (γ P Q i) "(#Hsts & Hγ & #HQ & HQR)".
   iMod (sts_openS (barrier_inv l P) _ _ γ with "[Hγ]")
     as ([p I]) "(% & [Hl Hr] & Hclose)"; eauto.
   iMod (saved_prop_alloc_strong (R1: ∙%CF (iProp Σ)) I) as (i1) "[% #Hi1]".
